src/Std/Data/DHashMap/Internal/List/Associative.lean
@@ -1861,18 +1861,6 @@ theorem length_alterKey [BEq α] [LawfulBEq α] {k : α} {f : Option (β k) → 
   cases h : getValueCast? k l <;> split <;> simp_all [length_eraseKey, length_insertEntry,
     containsKey_eq_isSome_getValueCast?, ← getValueCast?_eq_some_getValueCast]
 
-theorem isEmpty_alterKey [BEq α] [LawfulBEq α] {k : α} {f : Option (β k) → Option (β k)}
-    {l : List ((a : α) × β a)} :
-    (alterKey k f l).isEmpty ↔ (eraseKey k l).isEmpty ∧ f (getValueCast? k l) = none := by
-  simp only [alterKey, List.isEmpty_eq_true]
-  split
-  · next heq =>
-    simp only [iff_self_and, heq];
-    intros; trivial
-  · next heq =>
-    rw [heq, ← List.isEmpty_iff, isEmpty_insertEntry]
-    simp
-
 theorem alterKey_of_perm [BEq α] [LawfulBEq α] {a : α} {f : Option (β a) → Option (β a)}
     {l l' : List ((a : α) × β a)} (hl : DistinctKeys l) (hp : Perm l l') :
     Perm (alterKey a f l) (alterKey a f l') := by
@@ -1928,14 +1916,6 @@ theorem modifyKey_eq_alterKey [BEq α] [LawfulBEq α] (k : α) (f : β k → β 
   rw [modifyKey, alterKey, Option.map.eq_def]
   split <;> next h =>
     simp [h, insertEntry, containsKey_eq_isSome_getValueCast?, eraseKey_of_containsKey_eq_false]
-
-theorem isEmpty_modifyKey [BEq α] [LawfulBEq α] (k : α) (f : β k → β k)
-    (l : List ((a : α) × β a)) : (modifyKey k f l).isEmpty ↔ l.isEmpty := by
-  match l with
-  | [] => simp [modifyKey]
-  | a :: as =>
-    simp only [modifyKey, replaceEntry, cond_eq_if]
-    repeat' split <;> simp
 
 theorem mem_replaceEntry_of_key_ne [BEq α] [LawfulBEq α] {a : α} {b : β a}
     {l : List ((a : α) × β a)} (p : (a : α) × β a) (hne : p.1 ≠ a) :
@@ -2096,8 +2076,8 @@ theorem mem_eraseKey_of_key_ne [BEq α] [EquivBEq α] {a : α}
     · next h =>
       simp only [List.mem_cons, ih]
 
-theorem mem_alterKey_of_key_not_beq {β : Type v} [BEq α] [EquivBEq α] {a : α} {f : Option β → Option β}
-    {l : List ((_ : α) × β)} (p : (_ : α) × β) (hne : ¬(p.1 == a)) :
+theorem mem_alterKey_of_key_not_beq {β : Type v} [BEq α] [EquivBEq α] {a : α}
+    {f : Option β → Option β} {l : List ((_ : α) × β)} (p : (_ : α) × β) (hne : ¬(p.1 == a)) :
     p ∈ alterKey a f l ↔ p ∈ l := by
   rw [alterKey]
   split <;> simp only [mem_eraseKey_of_key_ne p hne, mem_insertEntry_of_key_ne p hne]
@@ -2134,8 +2114,9 @@ theorem containsKey_modifyKey_iff [BEq α] [EquivBEq α] (k : α) (f : β → β
 
 end Const
 
-theorem DistinctKeys.constAlterKey {β : Type v} [BEq α] [EquivBEq α] {a : α} {f : Option β → Option β}
-    {l : List ((_ : α) × β)} (hl : DistinctKeys l) : DistinctKeys (List.Const.alterKey a f l) := by
+theorem DistinctKeys.constAlterKey {β : Type v} [BEq α] [EquivBEq α] {a : α}
+    {f : Option β → Option β} {l : List ((_ : α) × β)} (hl : DistinctKeys l) :
+    DistinctKeys (List.Const.alterKey a f l) := by
   dsimp only [List.Const.alterKey]
   split
   · exact DistinctKeys.eraseKey hl
